Introduce tighter constraints on benumerate by introducing a bcount predicate
Assuming decidable equality on TItem, bags are now required to keep
track of how many times each items appear; the count function is not
required to be efficient though, since it mostly serves to assert
properties about the behaviour of binsert and benumerate.

The two interesting predicates are
  forall item, bcount beq bempty item = 0
and
  bcount beq (binsert container inserted) item =
  bcount beq container item + (if beq item inserted then 1 else 0).
where beq designates decidable equality.

The three existing implementations of bag have been augmented to show
that they conform to this extended interface.

src/QueryStructure/Refinements/Bags/BagsInterface.v
@@ -2,6 +2,9 @@ Require Export Program SetEq SetEqProperties.
 
 Unset Implicit Arguments.
 
+Definition HasDecidableEquality (T: Type) :=
+  forall (x y: T), {x = y} + {x <> y}.
+
 Definition BagInsertEnumerate
            {TContainer TItem: Type}
            (benumerate : TContainer -> list TItem)
@@ -9,12 +12,30 @@ Definition BagInsertEnumerate
   forall item inserted container,
     List.In item (benumerate (binsert container inserted)) <->
     List.In item (benumerate container) \/ item = inserted.
-    
+
+Definition BagInsertCount
+           {TContainer TItem}
+           (benumerate : TContainer -> list TItem)
+           (binsert    : TContainer -> TItem -> TContainer)
+           (bcount     : HasDecidableEquality TItem -> TContainer -> TItem -> nat) :=
+  forall (beq : HasDecidableEquality TItem),
+  forall item inserted container,
+    bcount beq (binsert container inserted) item =
+    bcount beq container item + (if beq item inserted then 1 else 0).
+
 Definition BagEnumerateEmpty
            {TContainer TItem: Type}
            (benumerate : TContainer -> list TItem)
            (bempty     : TContainer) :=
   forall item, ~ List.In item (benumerate bempty).
+
+Definition BagCountEmpty
+           {TContainer TItem: Type}
+           (benumerate : TContainer -> list TItem)
+           (bempty     : TContainer)
+           (bcount     : HasDecidableEquality TItem -> TContainer -> TItem -> nat) :=
+  forall (beq : HasDecidableEquality TItem),
+  forall item, bcount beq bempty item = 0. 
 
 Definition BagFindStar
            {TContainer TItem TSearchTerm: Type}
@@ -42,9 +63,12 @@ Class Bag (TContainer TItem TSearchTerm: Type) :=
     benumerate : TContainer -> list TItem;
     bfind      : TContainer -> TSearchTerm -> list TItem;
     binsert    : TContainer -> TItem -> TContainer;
-    
+    bcount     : HasDecidableEquality TItem -> TContainer -> TItem -> nat;
+
     binsert_enumerate : BagInsertEnumerate benumerate binsert;
+    binsert_count     : BagInsertCount benumerate binsert bcount;
     benumerate_empty  : BagEnumerateEmpty benumerate bempty;
+    bcount_empty      : BagCountEmpty benumerate bempty bcount;
     bfind_star        : BagFindStar bfind benumerate bstar;
     bfind_correct     : BagFindCorrect bfind bfind_matcher benumerate
   }.
