src/QueryStructure/Refinements/Bags/ListBags.v
@@ -13,6 +13,17 @@ Definition ListAsBag_binsert
            (item: TItem) :=
   cons item container.
 
+Fixpoint ListAsBag_bcount
+           {TItem: Type}
+           (beq : HasDecidableEquality TItem)
+           (container: list TItem)
+           (item: TItem) :=
+  match container with
+    | nil            => 0 
+    | cons head tail => (if beq item head then 1 else 0) 
+                      + ListAsBag_bcount beq tail item
+  end.
+
 Lemma List_BagInsertEnumerate :
   forall {TItem: Type},
   BagInsertEnumerate id (ListAsBag_binsert (TItem := TItem)).
@@ -20,6 +31,27 @@ Proof.
   firstorder.
 Qed.
 
+Lemma List_BagInsertCount :
+  forall {TItem: Type},
+    BagInsertCount (@id (list TItem)) ListAsBag_binsert ListAsBag_bcount.
+Proof.
+  compute; firstorder.
+Qed.
+
+Lemma List_BagEnumerateEmpty :
+  forall {TItem: Type},
+    BagEnumerateEmpty id (@nil TItem).
+Proof.
+  firstorder.
+Qed.
+
+Lemma List_BagCountEmpty :
+  forall {TItem},
+    BagCountEmpty (@id (list TItem)) nil ListAsBag_bcount.
+Proof.
+  firstorder.
+Qed.
+  
 Lemma List_BagFindStar :
   forall {TItem TSearchTerm: Type}
          (star: TSearchTerm)
@@ -32,13 +64,6 @@ Proof.
   [ | rewrite find_star, IHcontainer]; trivial.
 Qed.
 
-Lemma List_BagEnumerateEmpty :
-  forall {TItem: Type},
-    BagEnumerateEmpty id (@nil TItem).
-Proof.
-  firstorder.
-Qed.
-  
 Lemma List_BagFindCorrect :
   forall {TItem TSearchTerm: Type}
          (matcher: TSearchTerm -> TItem -> bool),
@@ -62,7 +87,9 @@ Instance ListAsBag
     binsert    := ListAsBag_binsert;
     
     binsert_enumerate := List_BagInsertEnumerate;
+    binsert_count     := List_BagInsertCount;
     benumerate_empty  := List_BagEnumerateEmpty;
+    bcount_empty      := List_BagCountEmpty;
     bfind_star        := List_BagFindStar star matcher find_star;
     bfind_correct     := List_BagFindCorrect matcher
   |}.
